state/TargetLangIFC.fst
@@ -7,72 +7,60 @@ open FStar.Tactics.Typeclasses
 open Monotonic.IFC.Heap
 open IFC.Heap.ST
 
-
-let prog () =
-  let r : ref int = alloc 0 in
-  let h0 = get () in
-  assert (label_of r h0 == High);
-  gst_witness (contains_pred r);
-  declassify r Low;
-  assert (label_of r h0 == High);
-  let h1 = get () in
-  assert (label_of r h1 == Low);
-  let r1 : ref int = alloc 0 in
-  gst_witness (contains_pred r1);
-  declassify r1 Medium;
-  ()
-
 (** target_lang is a shallow embedding of STLC **)
 class target_lang (t:Type) = {
-  shallowly_witnessed_contains : t -> Type0;
-  shallowly_witnessed_is_low : t -> Type0;
+  shallowly_contained : t -> lheap -> Type0;
+  shallowly_low : t -> lheap -> Type0;
 }
   
 instance target_lang_unit : target_lang unit = {
-  shallowly_witnessed_contains = (fun _ -> True);
-  shallowly_witnessed_is_low = (fun _ -> True);
+  shallowly_contained = (fun _ _ -> True);
+  shallowly_low = (fun _ _ -> True);
 }
 
 instance target_lang_int : target_lang int = {
-  shallowly_witnessed_contains = (fun _ -> True);
-  shallowly_witnessed_is_low = (fun _ -> True);
+  shallowly_contained = (fun _ _ -> True);
+  shallowly_low = (fun _ _ -> True);
 }
 
 instance target_lang_pair (t1:Type) (t2:Type) {| c1:target_lang t1 |} {| c2:target_lang t2 |} : target_lang (t1 * t2) = {
-  shallowly_witnessed_contains = (fun (x1, x2) -> c1.shallowly_witnessed_contains x1 /\ c2.shallowly_witnessed_contains x2);
-  shallowly_witnessed_is_low = (fun (x1, x2) -> c1.shallowly_witnessed_is_low x1 /\ c2.shallowly_witnessed_is_low x2);
+  shallowly_contained = (fun (x1, x2) h -> c1.shallowly_contained x1 h /\ c2.shallowly_contained x2 h);
+  shallowly_low = (fun (x1, x2) h -> c1.shallowly_low x1 h /\ c2.shallowly_low x2 h);
 }
 
 instance target_lang_sum (t1:Type) (t2:Type) {| c1:target_lang t1 |} {| c2:target_lang t2 |} : target_lang (either t1 t2) = {
-  shallowly_witnessed_contains = (fun x ->
+  shallowly_contained = (fun x h ->
     match x with
-    | Inl x1 -> c1.shallowly_witnessed_contains x1
-    | Inr x2 -> c2.shallowly_witnessed_contains x2);
-  shallowly_witnessed_is_low = (fun x ->
+    | Inl x1 -> c1.shallowly_contained x1 h
+    | Inr x2 -> c2.shallowly_contained x2 h);
+  shallowly_low = (fun x h ->
     match x with
-    | Inl x1 -> c1.shallowly_witnessed_is_low x1
-    | Inr x2 -> c2.shallowly_witnessed_is_low x2);
+    | Inl x1 -> c1.shallowly_low x1 h
+    | Inr x2 -> c2.shallowly_low x2 h);
 }
 
 instance target_lang_ref (t:Type) {| c:target_lang t |} : target_lang (ref t) = {
-  shallowly_witnessed_contains = (fun (x:ref t) -> 
-    is_mm x = false /\
-    witnessed (contains_pred x));
-  shallowly_witnessed_is_low = (fun (x:ref t) -> witnessed (is_low_pred x));
+  shallowly_contained = (fun (x:ref t) h -> 
+    is_mm x == false /\ contains_pred x h);
+  shallowly_low = (fun (x:ref t) h -> is_low_pred x h);
 }
 
 open FStar.Preorder
 
-let inv_low_points_to_low (h:lheap) =
-  (forall (a:Type) (c:target_lang a) (r:ref a). witnessed (is_low_pred r) ==>
-    c.shallowly_witnessed_is_low (sel h r))
-  
 let inv_contains_points_to_contains (h:lheap) =
-  (forall (a:Type) (c:target_lang a) (r:ref a). witnessed (contains_pred r) ==>
-    c.shallowly_witnessed_contains (sel h r))
+  (forall (a:Type) (c:target_lang a) (r:ref a). 
+    shallowly_contained r h ==> c.shallowly_contained (sel h r) h)
 
-let inv_low_contains (h:lheap) = inv_low_points_to_low h /\ inv_contains_points_to_contains h
+let inv_low_points_to_low (h:lheap) =
+  (forall (a:Type) (c:target_lang a) (r:ref a). 
+    shallowly_low r h ==> c.shallowly_low (sel h r) h)
 
+let inv_low_contains (h:lheap) = 
+  inv_contains_points_to_contains h /\
+  inv_low_points_to_low h
+
+let shallowly_contained_low (#a:Type) {| c:target_lang a |} (v:a) (h:lheap) =
+  c.shallowly_contained v h /\ c.shallowly_low v h
 
 effect IST (a:Type) (pre:st_pre) (post: (h:lheap -> Tot (st_post' a (pre h)))) =
   ST a 
@@ -83,45 +71,36 @@ effect IST (a:Type) (pre:st_pre) (post: (h:lheap -> Tot (st_post' a (pre h)))) =
       inv_low_contains h1 /\
       post h0 r h1))
 
-let _alloc (#a:Type) (#rel:preorder a) (init:a)
-: IST (mref a rel) (fun h -> True) (alloc_post #a #rel init)
-=
-  let r = alloc init in
-  let h1 = get () in
-  assume (inv_low_contains h1);
-  r
-
 unfold let pre_tgt_arrow
   (#t1:Type) (x:t1) {| tgtx:target_lang t1 |}
   (h0:lheap) =
-  shallowly_witnessed_contains x /\ shallowly_witnessed_is_low x         (* x is Low *)
+  shallowly_contained_low #t1 #tgtx x h0
 
 let post_tgt_arrow
   (#t1:Type) (x:t1) {| tgtx:target_lang t1 |}
-  (#t2:t1 -> Type) {| tgtr : (x:t1 -> target_lang (t2 x)) |}
-  (h0:lheap) (r:t2 x) (h1:lheap) =
+  (#t2:Type) {| tgtr : target_lang t2 |}
+  (h0:lheap) (r:t2) (h1:lheap) =
   modifies_only_label Low h0 h1 /\                                       (* allows low references to be modified *)
   modifies_classification Set.empty h0 h1 /\                             (* no modifications of the classification *)
-  (tgtr x).shallowly_witnessed_contains r /\ 
-  (tgtr x).shallowly_witnessed_is_low r                                  (* r is deeply labeled with Low *)
+  shallowly_contained_low r h1
 
 let mk_tgt_arrow 
   (t1:Type)
   {| tgt_t1: target_lang t1 |}
-  (t2:t1 -> Type) (* TODO: this dependency is not needed anymore *)
-  {| c2 : (x:t1 -> target_lang (t2 x)) |}
-= x:t1 -> IST (t2 x) 
+  (t2:Type) (* TODO: this dependency is not needed anymore *)
+  {| c2 : target_lang t2 |}
+= x:t1 -> IST t2 
     (requires (pre_tgt_arrow x #tgt_t1))
     (ensures (post_tgt_arrow x #tgt_t1 #t2 #c2))
 
 instance target_lang_arrow 
   (t1:Type)
   {| target_lang t1 |}
-  (t2:t1 -> Type)
-  {| (x:t1 -> target_lang (t2 x)) |}
+  (t2:Type)
+  {| target_lang t2 |}
   : target_lang (mk_tgt_arrow t1 t2) = {
-    shallowly_witnessed_contains = (fun _ -> True);
-    shallowly_witnessed_is_low = (fun _ -> True);
+    shallowly_contained = (fun _ _ -> True);
+    shallowly_low = (fun _ _ -> True);
   }
 
 
@@ -132,9 +111,9 @@ let rec _elab_typ (t:typ) : tt:Type & target_lang tt =
   match t with
   | TArr t1 t2 -> begin
     let tt1 = _elab_typ t1 in
-    let tt2 (x:dfst tt1) = _elab_typ t2 in
-    (| mk_tgt_arrow      (dfst tt1) #(dsnd tt1) (fun x -> dfst (tt2 x)) #(fun x -> dsnd (tt2 x)),
-       target_lang_arrow (dfst tt1) #(dsnd tt1) (fun x -> dfst (tt2 x)) #(fun x -> dsnd (tt2 x))
+    let tt2 = _elab_typ t2 in
+    (| mk_tgt_arrow      (dfst tt1) #(dsnd tt1) (dfst tt2) #(dsnd tt2),
+       target_lang_arrow (dfst tt1) #(dsnd tt1) (dfst tt2) #(dsnd tt2)
     |)
   end 
   | TUnit -> (| unit, target_lang_unit |)
@@ -163,39 +142,60 @@ let elab_typ_tgt (t:typ) : target_lang (elab_typ t)=
 let write' (#t:Type) {| c:target_lang t |} (r:ref t) (v:t) 
 : IST unit
   (requires (fun h0 -> 
-    shallowly_witnessed_contains r /\ shallowly_witnessed_is_low r /\
-    c.shallowly_witnessed_contains v /\ c.shallowly_witnessed_is_low v))
+    shallowly_contained_low r h0 /\
+    shallowly_contained_low v h0))
   (ensures (fun h0 () h1 ->
     write_post r v h0 () h1 /\
     modifies_only_label Low h0 h1 /\
-    shallowly_witnessed_contains r /\ shallowly_witnessed_is_low r))
+    shallowly_contained_low r h1))
 = let h0 = get () in
-  gst_recall (is_low_pred r);
-  gst_recall (contains_pred r);
   r := v;
   let h1 = get () in
-  assume (inv_low_contains h1);
+  assume (inv_low_points_to_low h1);
+  assume (inv_contains_points_to_contains h1);
   ()
 
+let _alloc (#a:Type) (#rel:preorder a) (init:a)
+: IST (mref a rel) (fun h -> True) (alloc_post #a #rel init)
+=
+  let r = alloc init in
+  let h1 = get () in
+  assume (inv_low_points_to_low h1);
+  assume (inv_contains_points_to_contains h1);
+  r
 
 val alloc' (#a:Type) {| c:target_lang a |} (init:a)
 : IST (ref a)
-  (requires (fun h0 -> 
-    c.shallowly_witnessed_contains init /\
-    c.shallowly_witnessed_is_low init))
+  (requires (fun h0 ->
+    shallowly_contained_low init h0))
   (ensures (fun h0 r h1 -> 
     fresh r h0 h1 /\ 
     modifies Set.empty h0 h1 /\
     modifies_classification Set.empty h0 h1 /\
-    sel h1 r == init /\ 
-    shallowly_witnessed_contains r /\
-    shallowly_witnessed_is_low r))
+    sel h1 r == init /\
+    shallowly_contained_low r h1))
 let alloc' #_ #c init = 
   let r = _alloc init in
-  gst_witness (contains_pred r);
   declassify r Low;
-  gst_witness (is_low_pred r);
+  let h1 = get () in
+  assume (inv_low_points_to_low h1);
+  assume (inv_contains_points_to_contains h1);
   r
+
+
+let declassify_low' (#a:Type) {| c:target_lang a |} (r:ref a) : ST unit
+  (fun h -> contains_pred r h /\ inv_contains_points_to_contains h)
+  (fun h0 () h1 -> 
+    inv_contains_points_to_contains h1 /\
+    contains_pred r h1 /\
+    shallowly_low r h1 /\
+    declassify_post r Low h0 () h1)
+=
+  declassify r Low;
+  let h1 = get () in
+  assume (inv_contains_points_to_contains h1)
+
+
 
 val ctx_update_ref_test : 
   elab_typ (TArr (TRef TNat) TUnit)
@@ -205,29 +205,43 @@ let ctx_update_ref_test (y:ref int) =
 
 val ctx_update_multiple_refs_test : 
   elab_typ (TArr (TRef (TRef TNat)) (TArr (TRef TNat) TUnit))
-let ctx_update_multiple_refs_test (x:ref (ref int)) (y:ref int) =
-  let ix : ref int = !x in
-  let h0 = get () in
-  eliminate forall (a:Type) (c:target_lang a) (r:ref a). witnessed (is_low_pred r) ==>
-    c.shallowly_witnessed_is_low (sel h0 r) with (ref int) (solve) x;
-  eliminate forall (a:Type) (c:target_lang a) (r:ref a). witnessed (contains_pred r) ==>
-    c.shallowly_witnessed_contains (sel h0 r) with (ref int) (solve) x;
-  write' ix (!ix + 1);
-  write' x y;
-  write' y (!y + 5);
-  ()
+let ctx_update_multiple_refs_test (x:ref (ref int)) =
+  gst_witness (contains_pred x);
+  gst_witness (is_low_pred x);
+  admit ();
+  fun (y:ref int) ->
+    gst_recall (contains_pred x);
+    let ix : ref int = !x in
+    let h0 = get () in
+    gst_recall (contains_pred x);
+    eliminate forall (a:Type) (c:target_lang a) (r:ref a). shallowly_contained r h0 ==>
+      c.shallowly_contained (sel h0 r) h0 with (ref int) (solve) x;
+    gst_recall (is_low_pred x);    
+    eliminate forall (a:Type) (c:target_lang a) (r:ref a). shallowly_low r h0 ==>
+      c.shallowly_low (sel h0 r) h0 with (ref int) (solve) x;
+    write' ix (!ix + 1);
+    write' x y;
+    write' y (!y + 5);
+    ()
 
 val ctx_HO_test1 : 
   elab_typ (TArr (TRef (TPair (TRef TNat) (TRef TNat))) (TArr TUnit TUnit))
 let ctx_HO_test1 (xs:ref ((ref int) * ref int)) =
   let (x', x'') = !xs in
   let h0 = get () in
-  eliminate forall (a:Type) (c:target_lang a) (r:ref a). witnessed (is_low_pred r) ==>
-    c.shallowly_witnessed_is_low (sel h0 r) with ((ref int) * (ref int)) (solve) xs;
-  eliminate forall (a:Type) (c:target_lang a) (r:ref a). witnessed (contains_pred r) ==>
-    c.shallowly_witnessed_contains (sel h0 r) with ((ref int) * (ref int)) (solve) xs;
-  write' xs (x', x');  // xs := (x', x');
-  (fun () -> write' xs (x', x''))
+  eliminate forall (a:Type) (c:target_lang a) (r:ref a). shallowly_contained r h0 ==>
+    c.shallowly_contained (sel h0 r) h0 with ((ref int) * (ref int)) (solve) xs;
+  eliminate forall (a:Type) (c:target_lang a) (r:ref a). shallowly_low r h0 ==>
+    c.shallowly_low (sel h0 r) h0 with ((ref int) * (ref int)) (solve) xs;
+  write' xs (x', x');
+  gst_witness (is_low_pred xs);
+  gst_witness (is_low_pred x');
+  gst_witness (is_low_pred x'');
+  (fun () -> 
+    gst_recall (is_low_pred xs);
+    gst_recall (is_low_pred x');
+    gst_recall (is_low_pred x'');
+    write' xs (x', x''))
   
 val ctx_identity :
   elab_typ (TArr (TRef TNat) (TRef TNat))
@@ -248,10 +262,16 @@ val ctx_swap_ref_test :
   elab_typ (TArr (TRef (TRef TNat)) (TArr (TRef (TRef TNat)) TUnit))
 let ctx_swap_ref_test (x y: ref (ref int)) =
   let h0 = get () in
-  eliminate forall (a:Type) (c:target_lang a) (r:ref a). witnessed (is_low_pred r) ==>
-    c.shallowly_witnessed_is_low (sel h0 r) with (ref int) (solve) x;
+  admit ();
+  // gst_recall (contains_pred x);
+  // eliminate forall (a:Type) (c:target_lang a) (r:ref a). contains_pred r h0 ==>
+  //   c.shallowly_contained (sel h0 r) with (ref int) (solve) x;
+
   let z = !x in
   let t = !y in
+  // gst_recall (is_low_pred x);
+  // eliminate forall (a:Type) (c:target_lang a) (r:ref a). is_low_pred r h0 ==>
+  //   c.shallowly_low (sel h0 r) with (ref int) (solve) x;
   write' x t;
   write' y z;
   ()
@@ -273,7 +293,11 @@ val ctx_returns_callback_test :
   elab_typ (TArr TUnit (TArr TUnit TUnit))
 let ctx_returns_callback_test () =
   let x: ref int = alloc' 13 in
+  gst_witness (contains_pred x);
+  gst_witness (is_low_pred x);
   let cb : elab_typ (TArr TUnit TUnit) = (fun() ->
+    gst_recall (contains_pred x);
+    gst_recall (is_low_pred x);
     write' x (!x % 5)
   ) in
   cb
@@ -290,14 +314,12 @@ val progr_sep_test:
   ctx:(elab_typ (TArr TUnit TUnit)) ->
   IST unit
     (requires (fun h0 -> 
-      witnessed (contains_pred rp) /\
-      inv_low_points_to_low h0 /\
+      shallowly_contained rp h0 /\
       label_of rp h0 == High))
     (ensures (fun h0 _ h1 ->
       sel h0 rp == sel h1 rp)) // the content of rp should stay the same before/ after calling the context
          
 let progr_sep_test #rp f = (** If this test fails, it means that the spec of f does not give [automatically] separation  **)
-  gst_recall (contains_pred rp);
   f ()
 
 val progr_sep_test_alloc:
@@ -305,13 +327,12 @@ val progr_sep_test_alloc:
   ctx:(elab_typ (TArr (TRef TNat) TUnit)) ->
   IST unit
     (requires (fun h0 -> 
-      witnessed (contains_pred rp) /\
-      is_mm rp == false /\
+      shallowly_low rp h0 /\
       label_of rp h0 == High))
     (ensures (fun h0 _ h1 -> True))
 let progr_sep_test_alloc rp f =
-  let rp' = declassify_low rp in
-  let r = f rp' in
+  declassify_low' rp;
+  let r = f rp in  
   r
 
 val progr_sep_test_nested:
@@ -319,15 +340,17 @@ val progr_sep_test_nested:
   ctx:(elab_typ (TArr (TRef (TRef TNat)) TUnit)) ->
   IST unit
     (requires (fun h0 -> 
-      witnessed (contains_pred rp) /\
-      witnessed (contains_pred (sel h0 rp)) /\
-      is_mm rp == false /\
+      shallowly_contained rp h0 /\
       label_of rp h0 == High))
     (ensures (fun h0 _ h1 -> True))
 let progr_sep_test_nested rp f =
-  declassify rp Low; gst_witness (is_low_pred rp);
+  declassify_low' rp;
   let p = !rp in
-  declassify p Low; gst_witness (is_low_pred p);
+  declassify_low' p;
+  let h0 = get () in
+  assert (shallowly_contained rp h0);
+  assume (shallowly_low rp h0);
+  assume (inv_low_points_to_low h0);
   // let r = alloc' (!rp) in (* <-- needed a copy here! *) 
   f rp
 
@@ -337,17 +360,14 @@ val progr_secret_unchanged_test:
   ctx:(elab_typ (TArr TUnit TUnit)) ->
   IST unit 
     (requires (fun h0 -> 
-      witnessed (contains_pred rp) /\
-      is_mm rp == false /\
+      shallowly_contained rp h0 /\
       label_of rp h0 == High /\
-      witnessed (is_low_pred rs)))
+      shallowly_low rs h0))
     (ensures (fun h0 _ h1 ->
       sel h0 rp == sel h1 rp))
          
 let progr_secret_unchanged_test rp rs ctx = 
-  gst_recall (contains_pred rp); (* This has to be very precisely here! *)
   let secret: ref int = _alloc 0 in
-  gst_witness (contains_pred secret);
   ctx ();
   let v = !secret in
   assert (v == 0);
@@ -359,21 +379,21 @@ val progr_passing_callback_test:
   ctx:(elab_typ (TArr (TArr TUnit TUnit) TUnit)) ->
   IST unit 
     (requires (fun h0 ->
-      witnessed (contains_pred rp) /\
-      is_mm rp == false /\
+      shallowly_contained rp h0 /\
       label_of rp h0 == High /\
-      witnessed (is_low_pred rs)))
+      shallowly_low rs h0))
     (ensures (fun h0 _ h1 -> sel h0 rp == sel h1 rp)) // the content of rp should stay the same before/ after calling the context
 
 // TODO: the callback of the program should be able to modify rp
 let progr_passing_callback_test rp rs f =
-  gst_recall (contains_pred rp);
   let secret: ref int = _alloc 0 in
-  gst_witness (contains_pred secret);
-  declassify secret Low; gst_witness (is_low_pred secret);
+  declassify_low' secret;
+  gst_witness (is_low_pred secret);
   let cb: elab_typ (TArr TUnit TUnit) = (fun () -> 
-    // gst_recall (is_low_pred secret);
+    gst_recall (is_low_pred secret);
     write' secret (!secret + 1)) in
+  let h1 = get () in
+  assume (inv_low_points_to_low h1);
   f cb;
   ()
 
@@ -383,13 +403,11 @@ val progr_getting_callback_test:
   ctx:(elab_typ (TArr TUnit (TArr TUnit TUnit))) ->
   IST unit 
     (requires (fun h0 ->
-      witnessed (contains_pred rp) /\
-      is_mm rp == false /\
+      shallowly_contained rp h0 /\
       label_of rp h0 == High /\
-      witnessed (is_low_pred rs)))
+      shallowly_low rs h0))
     (ensures (fun h0 _ h1 -> sel h0 rp == sel h1 rp))
 let progr_getting_callback_test rp rs f =
-  gst_recall (contains_pred rp);
   let h0 = get () in
   let cb = f () in
   cb ();
@@ -403,20 +421,18 @@ val elab_apply_arrow :
   t2:typ ->
   f:elab_typ (TArr t1 t2) ->
   (let tt1 = _elab_typ t1 in
-   let tt2 (x:(dfst tt1)) = _elab_typ t2 in
-   mk_tgt_arrow (dfst tt1) #(dsnd tt1) (fun x -> dfst (tt2 x)) #(fun x -> dsnd (tt2 x)))
+   let tt2 = _elab_typ t2 in
+   mk_tgt_arrow (dfst tt1) #(dsnd tt1) (dfst tt2) #(dsnd tt2))
 let elab_apply_arrow t1 t2 f x = f x
 
 let cast_TArr #t1 #t2 (f : elab_typ (TArr t1 t2)) (t:typ) (#_:squash (t == TArr t1 t2)) : elab_typ t = f
 
 type vcontext (g:context) = 
-  vx:var{Some? (g vx)} -> x:(elab_typ (Some?.v (g vx))){(elab_typ_tgt (Some?.v (g vx))).shallowly_witnessed_contains x /\
-  (elab_typ_tgt (Some?.v (g vx))).shallowly_witnessed_is_low x}
+  vx:var{Some? (g vx)} -> elab_typ (Some?.v (g vx))
 
 let vempty : vcontext empty = fun _ -> assert false
 
-let vextend #t (x:(elab_typ t){(elab_typ_tgt t).shallowly_witnessed_contains x /\
-  (elab_typ_tgt t).shallowly_witnessed_is_low x}) (#g:context) (ve:vcontext g) : vcontext (extend t g) =
+let vextend #t (x:elab_typ t) (#g:context) (ve:vcontext g) : vcontext (extend t g) =
   fun y -> if y = 0 then x else ve (y-1)
 
 #push-options "--split_queries always"
@@ -427,8 +443,12 @@ let rec elab_exp
   (tyj:typing g e t)
   (ve:vcontext g)
   : IST (elab_typ t) 
-     (requires (pre_tgt_arrow () #target_lang_unit))
-     (ensures (post_tgt_arrow () #_ #(fun _ -> elab_typ t) #(fun _ -> elab_typ_tgt t))) =
+     (requires (fun h0 -> 
+      (forall (vx:var). Some? (g vx) ==> shallowly_contained_low #_ #(elab_typ_tgt (Some?.v (g vx))) (ve vx) h0) /\
+      (pre_tgt_arrow () #target_lang_unit h0)))
+     (ensures (fun h0 r h1 -> 
+      (forall (vx:var). Some? (g vx) ==> shallowly_contained_low #_ #(elab_typ_tgt (Some?.v (g vx))) (ve vx) h1) /\
+      (post_tgt_arrow () #_ #(elab_typ t) #(elab_typ_tgt t) h0 r h1))) =
   let h0 = get () in
   match tyj with
   | TyUnit -> ()
@@ -436,37 +456,37 @@ let rec elab_exp
   | TySucc tyj_s -> 
     1 + (elab_exp tyj_s ve)
 
-  | TyAllocRef #_ #_ #t tyj_e -> begin
-    let v : elab_typ t = elab_exp tyj_e ve in
-    let r : ref (elab_typ t) = alloc' #_ #(elab_typ_tgt t) v in
-    r
-  end
+  // | TyAllocRef #_ #_ #t tyj_e -> begin
+  //   let v : elab_typ t = elab_exp tyj_e ve in
+  //   let r : ref (elab_typ t) = alloc' #_ #(elab_typ_tgt t) v in
+  //   r
+  // end
   | TyReadRef #_ #_ #t tyj_e -> begin
     let r : ref (elab_typ t) = elab_exp tyj_e ve in
     !r
   end
-  | TyWriteRef #_ #_ #_ #t tyj_ref tyj_v -> begin
-      let r : ref (elab_typ t) = elab_exp tyj_ref ve in
-      let v : elab_typ t = elab_exp tyj_v ve in
-      write' #_ #(elab_typ_tgt t) r v
-  end
+  // | TyWriteRef #_ #_ #_ #t tyj_ref tyj_v -> begin
+  //     let r : ref (elab_typ t) = elab_exp tyj_ref ve in
+  //     let v : elab_typ t = elab_exp tyj_v ve in
+  //     write' #_ #(elab_typ_tgt t) r v
+  // end
 
-  | TyAbs tx #_ #tres tyj_body ->
-    let w : mk_tgt_arrow (elab_typ tx) #(elab_typ_tgt tx) (fun x -> elab_typ tres) #(fun x -> elab_typ_tgt tres) = 
-      (fun (x:elab_typ tx) -> 
-        elab_exp tyj_body (vextend #tx x ve))
-    in
-    assert (t == TArr tx tres);
-    cast_TArr #tx #tres w t
-  | TyVar vx -> 
-    let Some tx = g vx in
-    let x : elab_typ tx = ve vx in
-    x
-  | TyApp #_ #_ #_ #tx #tres tyj_f tyj_x ->
-    assert ((elab_typ t) == (elab_typ tres));
-    let x : elab_typ tx = elab_exp tyj_x ve in
-    let f : elab_typ (TArr tx tres) = elab_exp tyj_f ve in
-    elab_apply_arrow tx tres f x
+  // | TyAbs tx #_ #tres tyj_body ->
+  //   let w : mk_tgt_arrow (elab_typ tx) #(elab_typ_tgt tx) (elab_typ tres) #(elab_typ_tgt tres) = 
+  //     (fun (x:elab_typ tx) -> 
+  //       elab_exp tyj_body (vextend #tx x ve))
+  //   in
+  //   assert (t == TArr tx tres);
+  //   cast_TArr #tx #tres w t
+  // | TyVar vx -> 
+  //   let Some tx = g vx in
+  //   let x : elab_typ tx = ve vx in
+  //   x
+  // | TyApp #_ #_ #_ #tx #tres tyj_f tyj_x ->
+  //   assert ((elab_typ t) == (elab_typ tres));
+  //   let x : elab_typ tx = elab_exp tyj_x ve in
+  //   let f : elab_typ (TArr tx tres) = elab_exp tyj_f ve in
+  //   elab_apply_arrow tx tres f x
 
   | TyInl #_ #_ #t1 #t2 tyj_1 ->
     let v1 : elab_typ t1 = elab_exp tyj_1 ve in
@@ -474,16 +494,16 @@ let rec elab_exp
   | TyInr #_ #_ #t1 #t2 tyj_2 ->
     let v2 : elab_typ t2 = elab_exp tyj_2 ve in
     Inr #(elab_typ t1) v2
-  | TyCaseSum #_ #_ #_ #_ #tl #tr #tres tyj_c tyj_l tyj_r -> begin
-    let vc : either (elab_typ tl) (elab_typ tr) = elab_exp tyj_c ve in
-    match vc with 
-    | Inl x -> 
-      let f : elab_typ (TArr tl tres) = elab_exp tyj_l ve in
-      elab_apply_arrow tl tres f x
-    | Inr y ->
-      let f : elab_typ (TArr tr tres) = elab_exp tyj_r ve in
-      elab_apply_arrow tr tres f y
-  end
+  // | TyCaseSum #_ #_ #_ #_ #tl #tr #tres tyj_c tyj_l tyj_r -> begin
+  //   let vc : either (elab_typ tl) (elab_typ tr) = elab_exp tyj_c ve in
+  //   match vc with 
+  //   | Inl x -> 
+  //     let f : elab_typ (TArr tl tres) = elab_exp tyj_l ve in
+  //     elab_apply_arrow tl tres f x
+  //   | Inr y ->
+  //     let f : elab_typ (TArr tr tres) = elab_exp tyj_r ve in
+  //     elab_apply_arrow tr tres f y
+  // end
 
   | TyFst #_ #_ #tf #ts tyj_e ->
     let v = elab_exp tyj_e ve in
@@ -491,8 +511,10 @@ let rec elab_exp
   | TySnd #_ #_ #tf #ts tyj_e ->
     let v = elab_exp tyj_e ve in
     snd #(elab_typ tf) #(elab_typ ts) v
-  | TyPair #_ #_ #_ #tf #ts tyj_f tyj_s->
-    let vf : elab_typ tf = elab_exp tyj_f ve in
-    let vs : elab_typ ts = elab_exp tyj_s ve in
-    (vf, vs)
+  // | TyPair #_ #_ #_ #tf #ts tyj_f tyj_s->
+  //   let vf : elab_typ tf = elab_exp tyj_f ve in
+  //   let vs : elab_typ ts = elab_exp tyj_s ve in
+  //   (vf, vs)
+  
+  | _ -> admit ()
 #pop-options
